CBV translation preservation

coq/CBV/cbv.sig
@@ -1,10 +1,15 @@
 type : Type
 bool : Type
+effect : Type
 Value : Type
 Exp : Type
 
+Tick : effect
+Add : effect -> effect -> effect
+Pure : effect
+
 Unit : type 
-Arr : type -> type -> type 
+Arr : type -> effect -> type -> type 
 Cross : type -> type -> type 
 Plus : type -> type -> type 
 
@@ -13,6 +18,7 @@ Lam : (Value -> Exp) -> Value
 Pair : Value -> Value -> Value 
 Inj: bool -> Value -> Value
 
+Tock : Exp
 Val : Value -> Exp 
 App : Exp -> Exp -> Exp 
 CaseS : Exp -> (Value -> Exp) -> (Value -> Exp) -> Exp
